some more heap modeling

src/ocaml-output/FStar_FStar.ml
@@ -103,16 +103,15 @@ in (match (opt) with
 let newDocs = (FStar_List.collect FStar_Extraction_ML_Code.doc_of_mllib mllibs)
 in (FStar_List.iter (fun _92_42 -> (match (_92_42) with
 | (n, d) -> begin
-(let _185_22 = (FStar_Options.prepend_output_dir (Prims.strcat n ext))
-in (let _185_21 = (FStar_Format.pretty (Prims.parse_int "120") d)
-in (FStar_Util.write_file _185_22 _185_21)))
+(let _185_21 = (FStar_Options.prepend_output_dir (Prims.strcat n ext))
+in (FStar_Util.write_file _185_21 (FStar_Format.pretty (Prims.parse_int "120") d)))
 end)) newDocs))
 end
 | Some ("Kremlin") -> begin
 (
 
-let programs = (let _185_23 = (FStar_List.map FStar_Extraction_Kremlin.translate mllibs)
-in (FStar_List.flatten _185_23))
+let programs = (let _185_22 = (FStar_List.map FStar_Extraction_Kremlin.translate mllibs)
+in (FStar_List.flatten _185_22))
 in (
 
 let bin = ((FStar_Extraction_Kremlin.current_version), (programs))
@@ -143,8 +142,8 @@ end
 end
 | FStar_Getopt.Success -> begin
 if ((FStar_Options.dep ()) <> None) then begin
-(let _185_25 = (FStar_Parser_Dep.collect FStar_Parser_Dep.VerifyAll filenames)
-in (FStar_Parser_Dep.print _185_25))
+(let _185_24 = (FStar_Parser_Dep.collect FStar_Parser_Dep.VerifyAll filenames)
+in (FStar_Parser_Dep.print _185_24))
 end else begin
 if (FStar_Options.interactive ()) then begin
 (
@@ -232,8 +231,8 @@ let _92_87 = (report_errors ())
 in (
 
 let _92_89 = (codegen (FStar_Util.Inr (((fmods), (env)))))
-in (let _185_26 = (FStar_All.pipe_right fmods (FStar_List.map FStar_Universal.module_or_interface_name))
-in (finished_message _185_26))))
+in (let _185_25 = (FStar_All.pipe_right fmods (FStar_List.map FStar_Universal.module_or_interface_name))
+in (finished_message _185_25))))
 end))
 end else begin
 (
@@ -247,8 +246,8 @@ let _92_95 = (report_errors ())
 in (
 
 let _92_97 = (codegen (FStar_Util.Inl (((fmods), (env)))))
-in (let _185_27 = (FStar_All.pipe_right fmods (FStar_List.map FStar_Stratified.module_or_interface_name))
-in (finished_message _185_27))))
+in (let _185_26 = (FStar_All.pipe_right fmods (FStar_List.map FStar_Stratified.module_or_interface_name))
+in (finished_message _185_26))))
 end))
 end)
 end else begin
@@ -293,13 +292,13 @@ end else begin
 ()
 end
 in if (FStar_Options.trace_error ()) then begin
-(let _185_32 = (FStar_Util.message_of_exn e)
-in (let _185_31 = (FStar_Util.trace_of_exn e)
-in (FStar_Util.print2_error "Unexpected error\n%s\n%s\n" _185_32 _185_31)))
+(let _185_31 = (FStar_Util.message_of_exn e)
+in (let _185_30 = (FStar_Util.trace_of_exn e)
+in (FStar_Util.print2_error "Unexpected error\n%s\n%s\n" _185_31 _185_30)))
 end else begin
 if (not (((FStar_Absyn_Util.handleable e) || (FStar_Syntax_Util.handleable e)))) then begin
-(let _185_33 = (FStar_Util.message_of_exn e)
-in (FStar_Util.print1_error "Unexpected error; please file a bug report, ideally with a minimized version of the source program that triggered the error.\n%s\n" _185_33))
+(let _185_32 = (FStar_Util.message_of_exn e)
+in (FStar_Util.print1_error "Unexpected error; please file a bug report, ideally with a minimized version of the source program that triggered the error.\n%s\n" _185_32))
 end else begin
 ()
 end
@@ -309,8 +308,8 @@ in (
 let _92_110 = (cleanup ())
 in (
 
-let _92_112 = (let _185_34 = (FStar_TypeChecker_Errors.report_all ())
-in (FStar_All.pipe_right _185_34 Prims.ignore))
+let _92_112 = (let _185_33 = (FStar_TypeChecker_Errors.report_all ())
+in (FStar_All.pipe_right _185_33 Prims.ignore))
 in (
 
 let _92_114 = (report_errors ())
