ulib/FStar.Array.fst
@@ -73,9 +73,9 @@ val swap: #a:Type -> x:array a -> i:nat -> j:nat{i <= j}
                             (ensures (fun h0 _u h1 ->
                                       (j < Seq.length (sel h0 x))
                                       /\ contains h1 x
-				      /\ modifies (only x) h0 h1))
-				      (* /\ sel h1 x == SeqProperties.swap (sel h0 x) i j)) *)
-                                      (* /\ (h1==Heap.upd h0 x (SeqProperties.swap (sel h0 x) i j)))) *)
+				      /\ modifies (only x) h0 h1
+				      /\ sel h1 x == FStar.SeqProperties.swap (sel h0 x) i j))
+                                      (* /\ (h1==Heap.upd h0 x (FStar.SeqProperties.swap (sel h0 x) i j)))) *)
 let swap #a x i j =
   let h0 = get () in
   let tmpi = index x i in
